Primitive_Matchers/Transform.thy
@@ -7,13 +7,13 @@ imports "Common_Primitive_Matcher"
 begin
 
 definition transform_strict :: "common_primitive rule list \<Rightarrow> common_primitive rule list" where 
-    "transform_strict = optimize_matches opt_MatchAny_match_expr(*^^10)*) \<circ> normalize_rules \<circ> optimize_matches optimize_primitive_univ \<circ> rw_Reject \<circ> rm_LogEmpty"
+    "transform_strict = optimize_matches opt_MatchAny_match_expr(*^^10)*) \<circ> normalize_rules_dnf \<circ> optimize_matches optimize_primitive_univ \<circ> rw_Reject \<circ> rm_LogEmpty"
 
 
 lemma assumes goodrs: "good_ruleset rs" and wf\<alpha>: "wf_unknown_match_tac \<alpha>"
       shows "(common_matcher, \<alpha>),p\<turnstile> \<langle>transform_strict rs, s\<rangle> \<Rightarrow>\<^sub>\<alpha> t \<longleftrightarrow> (common_matcher, \<alpha>),p\<turnstile> \<langle>rs, s\<rangle> \<Rightarrow>\<^sub>\<alpha> t"
       and "simple_ruleset (transform_strict rs)"
-      and "\<forall> r \<in> set (transform_strict rs). normalized_match (get_match r)"
+      and "\<forall> r \<in> set (transform_strict rs). normalized_nnf_match (get_match r)"
   proof -
     let ?\<gamma>="(common_matcher, \<alpha>)"
     let ?fw="\<lambda>rs. approximating_bigstep_fun ?\<gamma> p rs s"
@@ -25,15 +25,15 @@ lemma assumes goodrs: "good_ruleset rs" and wf\<alpha>: "wf_unknown_match_tac \<
     let ?rs3="(optimize_matches optimize_primitive_univ ?rs2)"
     from simple_rs2 optimize_matches_simple_ruleset have simple_rs3: "simple_ruleset ?rs3" by auto
 
-    let ?rs4="(normalize_rules ?rs3)"
-    from simple_rs3 simple_ruleset_normalize_rules have simple_rs4: "simple_ruleset ?rs4" by auto
+    let ?rs4="(normalize_rules_dnf ?rs3)"
+    from simple_rs3 simple_ruleset_normalize_rules_dnf have simple_rs4: "simple_ruleset ?rs4" by auto
     {fix rs::"'a rule list"
-      have "\<forall> r \<in> set (normalize_rules rs). normalized_match (get_match r)"
+      have "\<forall> r \<in> set (normalize_rules_dnf rs). normalized_nnf_match (get_match r)"
         apply(induction rs)
          apply(simp)
         apply(rename_tac r rs, case_tac r)
-        using normalized_match_normalize_match by fastforce
-      } hence normalized_rs4: "\<forall> r \<in> set (normalize_rules ?rs4). normalized_match (get_match r)" by auto
+        using normalized_nnf_match_normalize_match by fastforce
+      } hence normalized_rs4: "\<forall> r \<in> set (normalize_rules_dnf ?rs4). normalized_nnf_match (get_match r)" by auto
 
     let ?rs5="optimize_matches opt_MatchAny_match_expr ?rs4"
     from simple_rs4 optimize_matches_simple_ruleset have simple_rs5: "simple_ruleset ?rs5" by auto
@@ -48,7 +48,7 @@ lemma assumes goodrs: "good_ruleset rs" and wf\<alpha>: "wf_unknown_match_tac \<
       apply(rule optimize_matches[symmetric])
       using optimize_primitive_univ_correct_matchexpr by force
     also have "\<dots> = ?fw ?rs4"
-      apply(rule normalize_rules_correct[symmetric])
+      apply(rule normalize_rules_dnf_correct[symmetric])
       using simple_rs3 by (metis good_imp_wf_ruleset simple_imp_good_ruleset)
     also have "\<dots> = ?fw ?rs5" by (metis optimize_matches_opt_MatchAny_match_expr) 
     finally have rs: "?fw rs = ?fw ?rs5" .
@@ -58,7 +58,7 @@ lemma assumes goodrs: "good_ruleset rs" and wf\<alpha>: "wf_unknown_match_tac \<
     from simple_rs5 show "simple_ruleset (transform_strict rs)"
       by(simp add: transform_strict_def)
 
-    show "\<forall> r \<in> set (transform_strict rs). normalized_match (get_match r)"  oops
+    show "\<forall> r \<in> set (transform_strict rs). normalized_nnf_match (get_match r)"  oops
   (*qed*)
 
 end
