Output_Format/Format_Ln.thy
@@ -49,7 +49,7 @@ text{*append*}
   apply(simp add: alist_and_append NegPos_map_append bunch_of_lemmata_about_matches)
   by fastforce
 
-text{* assumes: @{const "normalized_match"}*}
+text{* assumes: @{const "normalized_nnf_match"}*}
 fun iptrule_match_collect :: "iptrule_match match_expr \<Rightarrow> match_Ln_uncompressed \<Rightarrow> match_Ln_uncompressed" where
   "iptrule_match_collect MatchAny accu = accu" |
   "iptrule_match_collect (Match (Src ip)) (UncompressedFormattedMatch src dst proto extra) = UncompressedFormattedMatch ((Pos ip)#src) dst proto extra" |
@@ -70,7 +70,7 @@ We can express @{const iptrule_match_collect} with @{const primitive_extractor}.
 Latter is more elegant.
 We keep the definition of @{const iptrule_match_collect} to show explicitly what we are doing here.
 *}
-lemma iptrule_match_collect_by_primitive_extractor: "normalized_match m \<Longrightarrow> iptrule_match_collect m (UncompressedFormattedMatch [] [] [] []) = (
+lemma iptrule_match_collect_by_primitive_extractor: "normalized_nnf_match m \<Longrightarrow> iptrule_match_collect m (UncompressedFormattedMatch [] [] [] []) = (
     let (srcs, m') = primitive_extractor (is_Src, src_range) m;
         (dsts, m'') = primitive_extractor (is_Dst, dst_range) m';
         (protos, m''') = primitive_extractor (is_Prot, prot_sel) m'';
@@ -93,7 +93,7 @@ text{*The empty @{const UncompressedFormattedMatch} always match*}
 lemma "matches \<gamma> (UncompressedFormattedMatch_to_match_expr (UncompressedFormattedMatch [] [] [] [])) a p"
   by(simp add: bunch_of_lemmata_about_matches)
 
-lemma UncompressedFormattedMatch_to_match_expr_correct: assumes "normalized_match m" and "matches \<gamma> (UncompressedFormattedMatch_to_match_expr accu) a p" shows
+lemma UncompressedFormattedMatch_to_match_expr_correct: assumes "normalized_nnf_match m" and "matches \<gamma> (UncompressedFormattedMatch_to_match_expr accu) a p" shows
   "matches \<gamma> (UncompressedFormattedMatch_to_match_expr (iptrule_match_collect m accu)) a p \<longleftrightarrow> matches \<gamma> m a p"
 using assms apply (induction m accu arbitrary: rule: iptrule_match_collect.induct)
   apply(case_tac [!] \<gamma>)
@@ -109,7 +109,7 @@ using assms apply (induction m accu arbitrary: rule: iptrule_match_collect.induc
   apply (simp add: eval_ternary_simps ip_in_ipv4range_set_from_bitmask_UNIV bunch_of_lemmata_about_matches)
   apply(simp add: matches_match_Ln_uncompressed_append bunch_of_lemmata_about_matches)
   (*the rest are the undefined cases*)
-  apply(simp_all) --{*@{text "\<not> normalized_match"}*}
+  apply(simp_all) --{*@{text "\<not> normalized_nnf_match"}*}
 done
 
 
@@ -117,7 +117,7 @@ done
 definition format_Ln_match :: "iptrule_match match_expr \<Rightarrow> match_Ln_uncompressed" where
   "format_Ln_match m \<equiv> iptrule_match_collect m (UncompressedFormattedMatch [] [] [] [])"
 
-corollary format_Ln_match_correct: "normalized_match m \<Longrightarrow> matches \<gamma> (UncompressedFormattedMatch_to_match_expr (format_Ln_match m)) a p \<longleftrightarrow> matches \<gamma> m a p"
+corollary format_Ln_match_correct: "normalized_nnf_match m \<Longrightarrow> matches \<gamma> (UncompressedFormattedMatch_to_match_expr (format_Ln_match m)) a p \<longleftrightarrow> matches \<gamma> m a p"
 unfolding format_Ln_match_def
 apply(rule UncompressedFormattedMatch_to_match_expr_correct)
  apply(assumption)
@@ -125,10 +125,10 @@ by(simp add: bunch_of_lemmata_about_matches)
 
 
 text{*We can also show the previous corollary by the correctness of @{const primitive_extractor}*}
-corollary "normalized_match m \<Longrightarrow> matches \<gamma> (UncompressedFormattedMatch_to_match_expr (format_Ln_match m)) a p \<longleftrightarrow> matches \<gamma> m a p"
+corollary "normalized_nnf_match m \<Longrightarrow> matches \<gamma> (UncompressedFormattedMatch_to_match_expr (format_Ln_match m)) a p \<longleftrightarrow> matches \<gamma> m a p"
 proof -
   {fix yc
-    have "normalized_match yc \<Longrightarrow> \<not> has_disc is_Dst yc \<Longrightarrow> \<not> has_disc is_Prot yc \<Longrightarrow> \<not> has_disc is_Extra yc \<Longrightarrow> \<not> has_disc is_Src yc \<Longrightarrow> matches \<gamma> yc a p"
+    have "normalized_nnf_match yc \<Longrightarrow> \<not> has_disc is_Dst yc \<Longrightarrow> \<not> has_disc is_Prot yc \<Longrightarrow> \<not> has_disc is_Extra yc \<Longrightarrow> \<not> has_disc is_Src yc \<Longrightarrow> matches \<gamma> yc a p"
     apply(induction yc)
     apply(simp_all add:bunch_of_lemmata_about_matches)
     apply(case_tac aa)
@@ -139,7 +139,7 @@ proof -
     apply(simp_all)
     done
   } note yc_exhaust=this
-  assume normalized: "normalized_match m" 
+  assume normalized: "normalized_nnf_match m" 
   {fix asrc msrc adst mdst aprot mprot aextra mextra
   from normalized have
       "primitive_extractor (is_Extra, extra_sel) mprot = (aextra, mextra) \<Longrightarrow>
@@ -165,7 +165,7 @@ qed
 
 
 
-lemma format_Ln_match_correct': "\<forall> m' \<in> set ms. normalized_match m' \<Longrightarrow> 
+lemma format_Ln_match_correct': "\<forall> m' \<in> set ms. normalized_nnf_match m' \<Longrightarrow> 
     approximating_bigstep_fun \<gamma> p (map (\<lambda>m. Rule m a) (map (\<lambda>m'. UncompressedFormattedMatch_to_match_expr (format_Ln_match m')) ms)) s =
     approximating_bigstep_fun \<gamma> p (map (\<lambda>m. Rule m a) ms) s"
 apply(rule match_list_semantics)
@@ -177,7 +177,7 @@ by (metis format_Ln_match_correct)
 
 
 definition format_Ln_rules_uncompressed :: "iptrule_match rule list \<Rightarrow> (match_Ln_uncompressed \<times> action) list" where
-  "format_Ln_rules_uncompressed rs = [((format_Ln_match (get_match r)), (get_action r)). r \<leftarrow> (normalize_rules rs)]"
+  "format_Ln_rules_uncompressed rs = [((format_Ln_match (get_match r)), (get_action r)). r \<leftarrow> (normalize_rules_dnf rs)]"
 
 definition Ln_rules_to_rule :: "(match_Ln_uncompressed \<times> action) list \<Rightarrow> iptrule_match rule list" where
   "Ln_rules_to_rule rs = [case r of (m,a) \<Rightarrow> Rule (UncompressedFormattedMatch_to_match_expr m) a. r \<leftarrow> rs]"
@@ -195,8 +195,8 @@ case (Cons r rs)
   have map_uncompressedmapping_simp: "\<And>ms a. (map ((\<lambda>(m, y). Rule (UncompressedFormattedMatch_to_match_expr m) y) \<circ> (\<lambda>r. (format_Ln_match (get_match r), get_action r)) \<circ> (\<lambda>m. Rule m a)) ms) =
        (map (\<lambda>m. Rule m a) (map (\<lambda>m'. UncompressedFormattedMatch_to_match_expr (format_Ln_match m')) ms))" by(simp)
 
-  let ?rsA="map ((\<lambda>(m, y). Rule (UncompressedFormattedMatch_to_match_expr m) y) \<circ> (\<lambda>r. (format_Ln_match (get_match r), get_action r))) (normalize_rules [r])"
-  let ?rsC="map ((\<lambda>(m, y). Rule (UncompressedFormattedMatch_to_match_expr m) y) \<circ> (\<lambda>r. (format_Ln_match (get_match r), get_action r))) (normalize_rules rs)"
+  let ?rsA="map ((\<lambda>(m, y). Rule (UncompressedFormattedMatch_to_match_expr m) y) \<circ> (\<lambda>r. (format_Ln_match (get_match r), get_action r))) (normalize_rules_dnf [r])"
+  let ?rsC="map ((\<lambda>(m, y). Rule (UncompressedFormattedMatch_to_match_expr m) y) \<circ> (\<lambda>r. (format_Ln_match (get_match r), get_action r))) (normalize_rules_dnf rs)"
   from approximating_bigstep_fun_wf_postpend[where rsB="[r]", simplified] have subst_rule:
     "\<And>rsA rsC. wf_ruleset \<gamma> p rsA \<Longrightarrow> wf_ruleset \<gamma> p [r] \<Longrightarrow>
     approximating_bigstep_fun \<gamma> p rsA s = approximating_bigstep_fun \<gamma> p [r] s \<Longrightarrow> approximating_bigstep_fun \<gamma> p (rsA @ rsC) s = approximating_bigstep_fun \<gamma> p (r # rsC) s"
@@ -204,16 +204,15 @@ case (Cons r rs)
   
   have "approximating_bigstep_fun \<gamma> p (Ln_rules_to_rule (format_Ln_rules_uncompressed (r # rs))) s = 
         approximating_bigstep_fun \<gamma> p
-             (map ((\<lambda>(m, y). Rule (UncompressedFormattedMatch_to_match_expr m) y) \<circ> (\<lambda>r. (format_Ln_match (get_match r), get_action r))) (normalize_rules (r # rs))) s"
+             (map ((\<lambda>(m, y). Rule (UncompressedFormattedMatch_to_match_expr m) y) \<circ> (\<lambda>r. (format_Ln_match (get_match r), get_action r))) (normalize_rules_dnf (r # rs))) s"
     by (simp add: Ln_rules_to_rule_def format_Ln_rules_uncompressed_def)
-  also have "... = approximating_bigstep_fun \<gamma> p (?rsA @ ?rsC) s" by(subst normalize_rules_fst, simp)
+  also have "... = approximating_bigstep_fun \<gamma> p (?rsA @ ?rsC) s" using normalize_rules_fst normalize_rules_dnf_def2 by (metis map_append) (*this is so broken \<dots>*)
   also have "... = approximating_bigstep_fun \<gamma> p (r # ?rsC) s" 
     proof(subst subst_rule)
       from Cons.prems good_ruleset_fst have "good_ruleset [r]" by fast
       hence "good_ruleset ?rsA"
        apply(cases r)
        apply(rename_tac m a,clarify)
-       apply(simp add: normalize_rules_singleton)
        apply(drule good_ruleset_normalize_match)
        apply(simp add: good_ruleset_alt)
        done
@@ -223,11 +222,10 @@ case (Cons r rs)
     next
       show "approximating_bigstep_fun \<gamma> p ?rsA s = approximating_bigstep_fun \<gamma> p [r] s"
        apply(case_tac r, rename_tac m a, clarify)
-       apply(simp add: normalize_rules_singleton)
        apply(simp add: map_uncompressedmapping_simp)
        apply(subst normalize_match_correct[symmetric])
        apply(subst format_Ln_match_correct'[symmetric])
-        apply(simp add: normalized_match_normalize_match)
+        apply(simp add: normalized_nnf_match_normalize_match)
        apply(simp)
        done
      next
