Primitive_Matchers/Primitive_Normalization.thy
@@ -31,7 +31,7 @@ text{*
   @{text primitive_extractor} filters the @{typ "'a match_expr"} and returns a tuple.
   The first element of the returned tuple is the filtered primitive matches, the second element is the remaining match expression.
 
-  It requires a @{const normalized_match}.
+  It requires a @{const normalized_nnf_match}.
   *}
 fun primitive_extractor :: "(('a \<Rightarrow> bool) \<times> ('a \<Rightarrow> 'b)) \<Rightarrow> 'a match_expr \<Rightarrow> ('b negation_type list \<times> 'a match_expr)" where
  "primitive_extractor _ MatchAny = ([], MatchAny)" |
@@ -55,9 +55,9 @@ text{*
 *}
 
 theorem primitive_extractor_correct: assumes 
-  "normalized_match m" and "wf_disc_sel (disc, sel) C" and "primitive_extractor (disc, sel) m = (as, ms)" 
+  "normalized_nnf_match m" and "wf_disc_sel (disc, sel) C" and "primitive_extractor (disc, sel) m = (as, ms)" 
   shows "matches \<gamma> (alist_and (NegPos_map C as)) a p \<and> matches \<gamma> ms a p \<longleftrightarrow> matches \<gamma> m a p"
-  and "normalized_match ms"
+  and "normalized_nnf_match ms"
   and "\<not> has_disc disc ms"
   and "\<forall>disc2. \<not> has_disc disc2 m \<longrightarrow> \<not> has_disc disc2 ms"
   and "\<forall>disc2 sel2. normalized_n_primitive (disc2, sel2) P m \<longrightarrow> normalized_n_primitive (disc2, sel2) P ms"
@@ -71,7 +71,7 @@ proof -
     apply(auto simp add: alist_and_append bunch_of_lemmata_about_matches)
     done
 
-  from assms(1) assm3' show "normalized_match ms"
+  from assms(1) assm3' show "normalized_nnf_match ms"
     apply(induction "(disc, sel)" m  arbitrary: as ms rule: primitive_extractor.induct)
           apply(simp)
          apply(simp)
@@ -111,7 +111,7 @@ proof -
 qed
 
 (*
-theorem primitive_extractor_correct': "normalized_match m \<Longrightarrow> wf_disc_sel discsel C \<Longrightarrow>
+theorem primitive_extractor_correct': "normalized_nnf_match m \<Longrightarrow> wf_disc_sel discsel C \<Longrightarrow>
   matches \<gamma> (alist_and (NegPos_map C (fst (primitive_extractor discsel m)))) a p \<and> matches \<gamma> (snd (primitive_extractor discsel m)) a p \<longleftrightarrow> matches \<gamma> m a p"
 apply(cases discsel)
 apply(drule primitive_extractor_correct)
@@ -124,7 +124,7 @@ text{*
 *}
 
 
-lemma primitive_extractor_normalized_helper: "normalized_match m \<Longrightarrow> (as, ms) = primitive_extractor discsel m \<Longrightarrow> normalized_match ms"
+lemma primitive_extractor_normalized_helper: "normalized_nnf_match m \<Longrightarrow> (as, ms) = primitive_extractor discsel m \<Longrightarrow> normalized_nnf_match ms"
   apply(induction discsel m  arbitrary: as ms rule: primitive_extractor.induct)
   apply(simp)
   apply(simp)
@@ -137,21 +137,21 @@ lemma primitive_extractor_normalized_helper: "normalized_match m \<Longrightarro
   apply(simp)
   done
   
-lemma primitive_extractor_normalized: "normalized_match m \<Longrightarrow> primitive_extractor (disc, sel) m = (as, ms) \<Longrightarrow> normalized_match ms"
+lemma primitive_extractor_normalized: "normalized_nnf_match m \<Longrightarrow> primitive_extractor (disc, sel) m = (as, ms) \<Longrightarrow> normalized_nnf_match ms"
 using primitive_extractor_normalized_helper by metis
 
 
 
-lemma primitive_extractor_has_disc_helper: "normalized_match m \<Longrightarrow> (as, ms) = primitive_extractor (disc, sel) m \<Longrightarrow> \<not> has_disc disc ms"
+lemma primitive_extractor_has_disc_helper: "normalized_nnf_match m \<Longrightarrow> (as, ms) = primitive_extractor (disc, sel) m \<Longrightarrow> \<not> has_disc disc ms"
   apply(induction "(disc, sel)" m  arbitrary: as ms rule: primitive_extractor.induct)
   apply(simp_all split: split_if_asm split_split_asm)
   done
 
-lemma primitive_extractor_has_disc: "normalized_match m \<Longrightarrow> primitive_extractor (disc, sel) m = (as, ms)\<Longrightarrow> \<not> has_disc disc ms"
+lemma primitive_extractor_has_disc: "normalized_nnf_match m \<Longrightarrow> primitive_extractor (disc, sel) m = (as, ms)\<Longrightarrow> \<not> has_disc disc ms"
 using primitive_extractor_has_disc_helper by metis
 
 
-lemma primitive_extractor_has_disc2_helper: "\<not> has_disc disc2 m \<Longrightarrow> normalized_match m \<Longrightarrow> (as, ms) = primitive_extractor (disc, sel) m \<Longrightarrow> \<not> has_disc disc2 ms"
+lemma primitive_extractor_has_disc2_helper: "\<not> has_disc disc2 m \<Longrightarrow> normalized_nnf_match m \<Longrightarrow> (as, ms) = primitive_extractor (disc, sel) m \<Longrightarrow> \<not> has_disc disc2 ms"
 apply(induction "(disc, sel)" m  arbitrary: as ms rule: primitive_extractor.induct)
 apply(simp)
 apply(simp split: split_if_asm)
@@ -161,7 +161,7 @@ apply(simp split: split_split_asm)
 apply(simp_all)
 done
 
-lemma primitive_extractor_has_disc2: "\<not> has_disc disc2 m \<Longrightarrow> normalized_match m \<Longrightarrow> primitive_extractor (disc, sel) m = (as, ms) \<Longrightarrow> \<not> has_disc disc ms \<and> \<not> has_disc disc2 ms"
+lemma primitive_extractor_has_disc2: "\<not> has_disc disc2 m \<Longrightarrow> normalized_nnf_match m \<Longrightarrow> primitive_extractor (disc, sel) m = (as, ms) \<Longrightarrow> \<not> has_disc disc ms \<and> \<not> has_disc disc2 ms"
 apply(rule conjI)
 using primitive_extractor_has_disc_helper apply(metis)
 using primitive_extractor_has_disc2_helper apply metis
@@ -169,16 +169,16 @@ done
 *)
 
 
-lemma primitive_extractor_matchesE: "wf_disc_sel (disc,sel) C \<Longrightarrow> normalized_match m \<Longrightarrow> primitive_extractor (disc, sel) m = (as, ms)
+lemma primitive_extractor_matchesE: "wf_disc_sel (disc,sel) C \<Longrightarrow> normalized_nnf_match m \<Longrightarrow> primitive_extractor (disc, sel) m = (as, ms)
   \<Longrightarrow>
-  (normalized_match ms \<Longrightarrow> \<not> has_disc disc ms \<Longrightarrow> (\<forall>disc2. \<not> has_disc disc2 m \<longrightarrow> \<not> has_disc disc2 ms) \<Longrightarrow> matches_other \<longleftrightarrow>  matches \<gamma> ms a p)
+  (normalized_nnf_match ms \<Longrightarrow> \<not> has_disc disc ms \<Longrightarrow> (\<forall>disc2. \<not> has_disc disc2 m \<longrightarrow> \<not> has_disc disc2 ms) \<Longrightarrow> matches_other \<longleftrightarrow>  matches \<gamma> ms a p)
   \<Longrightarrow>
   matches \<gamma> (alist_and (NegPos_map C as)) a p \<and> matches_other \<longleftrightarrow>  matches \<gamma> m a p"
 using primitive_extractor_correct by metis
 
-lemma primitive_extractor_matches_lastE: "wf_disc_sel (disc,sel) C \<Longrightarrow> normalized_match m \<Longrightarrow> primitive_extractor (disc, sel) m = (as, ms)
+lemma primitive_extractor_matches_lastE: "wf_disc_sel (disc,sel) C \<Longrightarrow> normalized_nnf_match m \<Longrightarrow> primitive_extractor (disc, sel) m = (as, ms)
   \<Longrightarrow>
-  (normalized_match ms \<Longrightarrow> \<not> has_disc disc ms \<Longrightarrow> (\<forall>disc2. \<not> has_disc disc2 m \<longrightarrow> \<not> has_disc disc2 ms) \<Longrightarrow> matches \<gamma> ms a p)
+  (normalized_nnf_match ms \<Longrightarrow> \<not> has_disc disc ms \<Longrightarrow> (\<forall>disc2. \<not> has_disc disc2 m \<longrightarrow> \<not> has_disc disc2 ms) \<Longrightarrow> matches \<gamma> ms a p)
   \<Longrightarrow>
   matches \<gamma> (alist_and (NegPos_map C as)) a p  \<longleftrightarrow>  matches \<gamma> m a p"
 using primitive_extractor_correct by metis
@@ -216,7 +216,7 @@ subsection{*Normalizing and Optimizing Primitives*}
   
   text{*
     If @{text f} has the properties described above, then @{const normalize_primitive_extract} is a valid transformation of a match expression*}
-  lemma normalize_primitive_extract: assumes "normalized_match m" and "wf_disc_sel disc_sel C" and
+  lemma normalize_primitive_extract: assumes "normalized_nnf_match m" and "wf_disc_sel disc_sel C" and
         "\<forall>ml. (match_list \<gamma> (map (Match \<circ> C) (f ml)) a p \<longleftrightarrow> matches \<gamma> (alist_and (NegPos_map C ml)) a p)"
         shows "match_list \<gamma> (normalize_primitive_extract disc_sel C f m) a p \<longleftrightarrow> matches \<gamma> m a p"
     proof -
@@ -232,18 +232,30 @@ subsection{*Normalizing and Optimizing Primitives*}
       finally show ?thesis by simp
     qed
 
+  thm match_list_semantics[of \<gamma> "(map (Match \<circ> C) (f ml))" a p "[(alist_and (NegPos_map C ml))]"]
+
+  corollary normalize_primitive_extract_semantics:  assumes "normalized_nnf_match m" and "wf_disc_sel disc_sel C" and
+        "\<forall>ml. (match_list \<gamma> (map (Match \<circ> C) (f ml)) a p \<longleftrightarrow> matches \<gamma> (alist_and (NegPos_map C ml)) a p)"
+        shows "approximating_bigstep_fun \<gamma> p (map (\<lambda>m. Rule m a) (normalize_primitive_extract disc_sel C f m)) s = 
+              approximating_bigstep_fun \<gamma> p [Rule m a] s"
+  proof -
+    from normalize_primitive_extract[OF assms(1) assms(2) assms(3)] have
+      "match_list \<gamma> (normalize_primitive_extract disc_sel C f m) a p = matches \<gamma> m a p" .
+    also have "\<dots> \<longleftrightarrow> match_list \<gamma> [m] a p" by simp
+    finally show ?thesis using match_list_semantics[of \<gamma> "(normalize_primitive_extract disc_sel C f m)" a p "[m]"] by simp
+  qed
 
   lemma normalize_primitive_extract_maintains_normalized:
-  assumes "normalized_match m"
+  assumes "normalized_nnf_match m"
       and "normalized_n_primitive (disc2, sel2) P m"
       and "wf_disc_sel (disc1, sel1) C"
       and "\<forall>a. \<not> disc2 (C a)" --"disc1 and disc2 match for different stuff. e.g. Src_Ports and Dst_Ports"
-    shows "\<forall>mn \<in> set (normalize_primitive_extract (disc1, sel1) C f m). normalized_n_primitive (disc2, sel2) P mn \<and> normalized_match mn"
+    shows "\<forall>mn \<in> set (normalize_primitive_extract (disc1, sel1) C f m). normalized_n_primitive (disc2, sel2) P mn \<and> normalized_nnf_match mn"
     proof
       fix mn
       assume assm2: "mn \<in> set (normalize_primitive_extract (disc1, sel1) C f m)"
       obtain as ms where as_ms: "primitive_extractor (disc1, sel1) m = (as, ms)" by fastforce
-      from as_ms primitive_extractor_correct[OF assms(1) assms(3)] have "normalized_match ms"
+      from as_ms primitive_extractor_correct[OF assms(1) assms(3)] have "normalized_nnf_match ms"
                   and "\<not> has_disc disc1 ms"
                   and "normalized_n_primitive (disc2, sel2) P ms"
         apply -
@@ -251,7 +263,7 @@ subsection{*Normalizing and Optimizing Primitives*}
         using assms(2) by(fast)
       from assm2 as_ms have normalize_primitive_extract_unfolded: "mn \<in> ((\<lambda>spt. MatchAnd (Match (C spt)) ms) ` set (f as))"
         unfolding normalize_primitive_extract_def by force
-      with `normalized_match ms` have "normalized_match mn" by fastforce
+      with `normalized_nnf_match ms` have "normalized_nnf_match mn" by fastforce
       
       from normalize_primitive_extract_unfolded obtain Casms where Casms: "mn = (MatchAnd (Match (C Casms)) ms)" (*and "Casms \<in> set (f as)"*) by blast
 
@@ -259,7 +271,7 @@ subsection{*Normalizing and Optimizing Primitives*}
         by(simp)
 
       with Casms have "normalized_n_primitive (disc2, sel2) P mn" by blast
-      with `normalized_match mn` show "normalized_n_primitive (disc2, sel2) P mn \<and> normalized_match mn" by simp
+      with `normalized_nnf_match mn` show "normalized_n_primitive (disc2, sel2) P mn \<and> normalized_nnf_match mn" by simp
     qed
 
 end
